stack example verified

examples/Stack/Stack_proof.v
@@ -7,19 +7,20 @@ Generalizable Variables A.
 Implicit Types n m : int.
 Implicit Types p q : loc.
 
-Require Import Stack_ml.
 
+Require Import Stack_ml.
+Require stack_valid.
 
 (* ********************************************************************** *)
 (** ** Representation predicate *)
 
 (** [p ~> Stack L] relates a pointer [p] with the list [L] made of
     the elements in the stack. *)
-
-Definition Stack A `{Enc A} (L:list A) (p:loc) : hprop :=
+Module Stack : stack_valid.T.
+Definition Stack (L:list int) (p:loc) : hprop :=
   p ~~> L.
 
-Lemma Stack_eq : forall (p:loc) A `{Enc A} (L:list A),
+Lemma Stack_eq : forall (p:loc) (L:list int),
   p ~> Stack L  =  p ~~> L.
 Proof using. auto. Qed.
 
@@ -27,10 +28,10 @@ Proof using. auto. Qed.
 (* ********************************************************************** *)
 (** ** Verification *)
 
-Lemma create_spec : forall A `{Enc A},
+Lemma create_spec : 
   SPEC (create tt)
     PRE \[]
-    POST (fun p => (p ~> Stack (@nil A))).
+    POST (fun p => (p ~> Stack nil)).
 Proof using.
   xcf. xapp. xsimpl.
   (* TODO: how to avoid the Unshelve? *)
@@ -39,7 +40,7 @@ Qed.
 
 Hint Extern 1 (RegisterSpec create) => Provide create_spec.
 
-Lemma is_empty_spec : forall A `{Enc A} (p:loc) (L:list A),
+Lemma is_empty_spec : forall (p:loc) (L:list int),
   SPEC (is_empty p)
     PRE (p ~> Stack L)
     POST (fun (b:bool) => \[b = isTrue (L = nil)] \* p ~> Stack L).
@@ -50,7 +51,7 @@ Qed.
 
 Hint Extern 1 (RegisterSpec is_empty) => Provide is_empty_spec.
 
-Lemma push_spec : forall A `{Enc A} (p:loc) (x:A) (L:list A),
+Lemma push_spec : forall (p:loc) (x:int) (L:list int),
   SPEC (push p x)
     PRE (p ~> Stack L)
     POSTUNIT (p ~> Stack (x::L)).
@@ -60,31 +61,31 @@ Qed.
 
 Hint Extern 1 (RegisterSpec push) => Provide push_spec.
 
-Lemma pop_spec : forall A `{Enc A} (p:loc) (L:list A),
+Lemma pop_spec : forall (p:loc) (L:list int),
   L <> nil ->
   SPEC (pop p)
     PRE (p ~> Stack L)
-    POST (fun (x:A) => \exists L', \[L = x::L'] \* (p ~> Stack L')).
+    POST (fun (x:int) => \exists L', \[L = x::L'] \* (p ~> Stack L')).
 Proof using.
   introv N. xcf. xunfold Stack. xmatch. { xapp. xvals*. }
 Qed.
 
 Hint Extern 1 (RegisterSpec pop) => Provide pop_spec.
 
-Lemma clear_spec : forall A `{Enc A} (p:loc) (L:list A),
+Lemma clear_spec : forall (p:loc) (L:list int),
   SPEC (clear p)
     PRE (p ~> Stack L)
-    POSTUNIT (p ~> Stack (@nil A)).
+    POSTUNIT (p ~> Stack nil).
 Proof using.
   xcf. xunfold Stack. xapp. xsimpl.
 Qed.
 
 Hint Extern 1 (RegisterSpec clear) => Provide clear_spec.
 
-Lemma concat_spec : forall A `{Enc A} (p1 p2:loc) (L1 L2:list A),
+Lemma concat_spec : forall (p1 p2:loc) (L1 L2:list int),
   SPEC (concat p1 p2)
     PRE (p1 ~> Stack L1 \* p2 ~> Stack L2)
-    POSTUNIT (p1 ~> Stack (L1 ++ L2) \* p2 ~> Stack (@nil A)).
+    POSTUNIT (p1 ~> Stack (L1 ++ L2) \* p2 ~> Stack nil).
 Proof using.
   xcf. xunfold Stack. xapp. xapp. xapp.
   rewrite <- (Stack_eq p2). xapp. xsimpl.
@@ -94,18 +95,29 @@ Hint Extern 1 (RegisterSpec concat) => Provide concat_spec.
 
 Opaque Stack.
 
-Lemma rev_append_spec : forall A `{Enc A} (p1 p2:loc) (L1 L2:list A),
+Lemma rev_append_spec : forall (p1 p2:loc) (L1 L2:list int),
   SPEC (rev_append p1 p2)
     PRE (p1 ~> Stack L1 \* p2 ~> Stack L2)
-    POSTUNIT (p1 ~> Stack (@nil A) \* p2 ~> Stack (rev L1 ++ L2)).
+    POSTUNIT (p1 ~> Stack nil \* p2 ~> Stack (rev L1 ++ L2)).
 Proof using.
-  intros. gen p1 p2 L2. induction_wf IH: (@list_sub A) L1. intros.
+intros. gen p1 p2 L2. induction_wf IH: list_sub L1. intros.
   xcf. xif; intros C.
   { (* case cons *)
     xapp~ ;=> x L1' E. xapp. xapp. { subst*. } xsimpl. subst. rew_list~. }
   { (* case nil *)
-    xval. xsimpl~. subst. rew_list~. }
+    xval. xsimpl~. subst. rew_list~. } 
 Qed.
+
 
 Hint Extern 1 (RegisterSpec rev_append) => Provide rev_append_spec.
 
+Definition create : val := Stack_ml.create.
+Definition is_empty := is_empty.
+Definition push := push.
+Definition pop := pop.
+Definition clear := clear.
+Definition concat := concat.
+Definition rev_append := rev_append.
+
+
+End Stack.
