examples/translations/Stack_valid/stack_valid.v
@@ -1,0 +1,179 @@
+(* Created module type
+   T -> Stack
+   CFML example is now monomorphic
+   Added aliases for ocaml functions
+   removed underscore from spec names
+   added hypothesis to pop
+   general inlining.
+   changed order of arguments.
+   removed redundant representation predicate Int.
+   changed is_empty so that it uses the isTrue predicate. 
+ *)
+
+Require Import Gospel.
+
+Require Coq.ZArith.BinInt TLC.LibLogic TLC.LibRelation TLC.LibInt TLC.LibListZ.
+
+Require Import CFML.SepBase CFML.SepLifted CFML.WPLib CFML.WPLifted CFML.WPRecord CFML.WPArray CFML.WPBuiltin.
+
+Require CFML.Stdlib.Array_ml CFML.Stdlib.List_ml CFML.Stdlib.Sys_ml.
+
+Require Import Coq.ZArith.BinIntDef CFML.Semantics CFML.WPHeader.
+
+Module Type T.
+Set Implicit Arguments.
+
+Parameter Stack :
+  Coq.Lists.List.list int ->
+  loc -> CFML.SepBase.SepBasicSetup.SepSimplArgsCredits.hprop.
+
+Parameter create : CFML.Semantics.val.
+
+Parameter create_spec :
+  CFML.SepLifted.Triple (
+    CFML.SepLifted.Trm_apps create (cons (@CFML.SepLifted.dyn_make unit _ tt) nil)
+  ) CFML.SepBase.SepBasicSetup.SepSimplArgsCredits.hempty (
+    fun _prog_p : loc =>
+        CFML.SepBase.SepBasicSetup.HS.repr (Stack nil) _prog_p
+    ). 
+
+Parameter is_empty : CFML.Semantics.val.
+
+Parameter is_empty_spec :
+  forall _prog_q : loc,
+  forall q : Coq.Lists.List.list int,
+  CFML.SepLifted.Triple (
+    CFML.SepLifted.Trm_apps is_empty (
+      Coq.Lists.List.cons (@CFML.SepLifted.dyn_make loc _ _prog_q) Coq.Lists.List.nil
+    )
+  ) (CFML.SepBase.SepBasicSetup.HS.repr (Stack q) _prog_q) (
+    fun b : bool =>
+      CFML.SepBase.SepBasicSetup.SepSimplArgsCredits.hstar (
+          CFML.SepBase.SepBasicSetup.SepSimplArgsCredits.hpure (
+              Coq.Init.Logic.eq b (isTrue(Coq.Init.Logic.eq q Coq.Lists.List.nil))
+            )
+
+        ) (
+          CFML.SepBase.SepBasicSetup.HS.repr (Stack q) _prog_q
+        )
+    ).
+  
+Parameter push : CFML.Semantics.val.
+
+Parameter push_spec :
+  forall _prog_p : loc,
+  forall x : int,    
+  forall p : Coq.Lists.List.list int,
+  CFML.SepLifted.Triple (
+    CFML.SepLifted.Trm_apps push (
+      Coq.Lists.List.cons (@CFML.SepLifted.dyn_make loc _ _prog_p) (
+        Coq.Lists.List.cons (@CFML.SepLifted.dyn_make int _ x) Coq.Lists.List.nil
+      )
+    )
+    ) (CFML.SepBase.SepBasicSetup.HS.repr (Stack p) _prog_p) (
+    fun _ : Coq.Init.Datatypes.unit =>
+      CFML.SepBase.SepBasicSetup.HS.repr (Stack (Coq.Lists.List.cons x p)) _prog_p
+  ).
+
+Parameter pop : CFML.Semantics.val.
+
+Parameter pop_spec :
+  forall _prog_p : loc,
+  forall p : Coq.Lists.List.list int,
+    p <> nil ->
+  CFML.SepLifted.Triple (
+    CFML.SepLifted.Trm_apps pop (
+      Coq.Lists.List.cons (@CFML.SepLifted.dyn_make loc _ _prog_p) Coq.Lists.List.nil
+    )
+  ) (CFML.SepBase.SepBasicSetup.HS.repr (Stack p) _prog_p) (
+    fun r : int =>
+    CFML.SepBase.SepBasicSetup.SepSimplArgsCredits.hexists (
+      fun _p' : Coq.Lists.List.list int =>
+        CFML.SepBase.SepBasicSetup.SepSimplArgsCredits.hstar
+          (
+            CFML.SepBase.SepBasicSetup.SepSimplArgsCredits.hpure (
+              Coq.Init.Logic.eq p (Coq.Lists.List.cons r _p')
+            )
+          )
+          (
+          CFML.SepBase.SepBasicSetup.HS.repr (Stack _p') _prog_p
+        )         
+      )
+    )
+  .
+
+Parameter clear : CFML.Semantics.val.
+
+Parameter clear_spec :
+  forall _prog_p : loc,
+  forall p : Coq.Lists.List.list int,
+  CFML.SepLifted.Triple (
+    CFML.SepLifted.Trm_apps clear (
+      Coq.Lists.List.cons (@CFML.SepLifted.dyn_make loc _ _prog_p) Coq.Lists.List.nil
+    )
+  ) (CFML.SepBase.SepBasicSetup.HS.repr (Stack p) _prog_p) (
+    fun _ : Coq.Init.Datatypes.unit =>
+      CFML.SepBase.SepBasicSetup.HS.repr (Stack Coq.Lists.List.nil) _prog_p  
+  ).
+
+Parameter concat : CFML.Semantics.val.
+
+
+Parameter concat_spec :
+  forall _prog_q1 : loc,
+  forall _prog_q2 : loc,
+  forall q1 : Coq.Lists.List.list int,    
+  forall q2 : Coq.Lists.List.list int,
+  CFML.SepLifted.Triple (
+    CFML.SepLifted.Trm_apps concat (
+      Coq.Lists.List.cons (@CFML.SepLifted.dyn_make loc _ _prog_q1) (
+        Coq.Lists.List.cons (@CFML.SepLifted.dyn_make loc _ _prog_q2) Coq.Lists.List.nil
+      )
+    )
+  ) (
+    CFML.SepBase.SepBasicSetup.SepSimplArgsCredits.hstar (
+      CFML.SepBase.SepBasicSetup.HS.repr (Stack q1) _prog_q1
+    ) (CFML.SepBase.SepBasicSetup.HS.repr (Stack q2) _prog_q2)
+  ) (
+    fun _ : Coq.Init.Datatypes.unit =>
+      CFML.SepBase.SepBasicSetup.SepSimplArgsCredits.hstar
+                        (
+            CFML.SepBase.SepBasicSetup.HS.repr (Stack (TLC.LibList.app q1 q2)) _prog_q1
+        )
+
+        (
+          CFML.SepBase.SepBasicSetup.HS.repr (Stack Coq.Lists.List.nil) _prog_q2
+        )
+
+      )
+  .
+
+Parameter rev_append : CFML.Semantics.val.
+
+Parameter rev_append_spec :
+  forall _prog_p1 : loc,
+  forall _prog_p2 : loc,
+  forall p1 : Coq.Lists.List.list int,
+  forall p2 : Coq.Lists.List.list int,
+  CFML.SepLifted.Triple (
+    CFML.SepLifted.Trm_apps rev_append (
+      Coq.Lists.List.cons (@CFML.SepLifted.dyn_make loc _ _prog_p1) (
+        Coq.Lists.List.cons (@CFML.SepLifted.dyn_make loc _ _prog_p2) Coq.Lists.List.nil
+      )
+    )
+  ) (
+    CFML.SepBase.SepBasicSetup.SepSimplArgsCredits.hstar (
+      CFML.SepBase.SepBasicSetup.HS.repr (Stack p1) _prog_p1
+    ) (CFML.SepBase.SepBasicSetup.HS.repr (Stack p2) _prog_p2)
+  ) (
+    fun _ : Coq.Init.Datatypes.unit =>
+        CFML.SepBase.SepBasicSetup.SepSimplArgsCredits.hstar (
+          CFML.SepBase.SepBasicSetup.HS.repr (Stack Coq.Lists.List.nil) _prog_p1
+        ) (
+            CFML.SepBase.SepBasicSetup.HS.repr (Stack (TLC.LibList.app (rev p1) p2)) _prog_p2
+    )
+  ).
+
+
+
+End T.
